Add support for abstract types
Co-authored-by: Benjamin Gregoire <Benjamin.Gregoire@inria.fr>

compiler/src/compile.ml
@@ -59,7 +59,7 @@ let warn_extra_fd pd asmOp (_, fd) = List.iter (warn_extra_i pd asmOp) fd.f_body
 let do_spill_unspill asmop ?(debug = false) cp =
   let p = Conv.cuprog_of_prog cp in
   match
-    Lower_spill.spill_uprog asmop
+    Lower_spill.spill_uprog Build_Tabstract asmop
       (fun k ii -> Conv.fresh_var_ident k ii (Uint63.of_int 0))
       p
   with
@@ -355,6 +355,6 @@ let compile (type reg regx xreg rflag cond asm_op extra_op)
       (snd prog) []
   in
 
-  Compiler.compile_prog_to_asm Arch.asm_e Arch.call_conv Arch.aparams cparams
+  Compiler.compile_prog_to_asm Build_Tabstract Arch.asm_e Arch.call_conv Arch.aparams cparams
     export_functions
-    (Expr.to_uprog Arch.asmOp cprog)
+    (Expr.to_uprog Build_Tabstract Arch.asmOp cprog)
