compiler/src/sct_checker_forward.ml
@@ -719,7 +719,8 @@ let expr_equal a b =
     | RISCV  -> Riscv_decl.riscv_fcp
   in 
   let normalize e =
-    e |> Conv.cexpr_of_expr |> Constant_prop.(const_prop_e fcp None empty_cpm) in
+    e |> Conv.cexpr_of_expr |> Constant_prop.(const_prop_e Build_Tabstract fcp None empty_cpm)
+  in
   Expr.eq_expr (normalize a) (normalize b)
 
 (* ------------------------------------------------------------- *)
