proofs/compiler/remove_globals_proof.v
@@ -6,15 +6,16 @@ Require Import xseq.
 Require Import compiler_util expr psem remove_globals low_memory.
 Import Utf8.
 
-Definition gd_incl (gd1 gd2: glob_decls) :=
+Definition gd_incl {tabstract : Tabstract} (gd1 gd2: glob_decls) :=
   forall g v, get_global gd1 g = ok v -> get_global gd2 g = ok v.
 
-Lemma gd_inclT gd3 gd1 gd2 :  gd_incl gd1 gd3 -> gd_incl gd3 gd2 -> gd_incl gd1 gd2.
+Lemma gd_inclT {tabstract : Tabstract} gd3 gd1 gd2 :  gd_incl gd1 gd3 -> gd_incl gd3 gd2 -> gd_incl gd1 gd2.
 Proof. by move=> h1 h2 g v /h1 /h2. Qed.
 
 Module INCL. Section INCL.
 
   Context
+    {tabstract : Tabstract}
     {wsw : WithSubWord}
     {dc:DirectCall}
     {asm_op syscall_state : Type}
@@ -311,6 +312,7 @@ End EXTEND. Import EXTEND.
 Module RGP. Section PROOFS.
 
   Context
+    {tabstract : Tabstract}
     {wsw : WithSubWord}
     {dc:DirectCall}
     {asm_op syscall_state : Type}
