proofs/compiler/dead_calls_proof.v
@@ -7,6 +7,7 @@ Import Utf8 xseq.
 Section WITH_PARAMS.
 
 Context
+  {tabstract : Tabstract}
   {wsw : WithSubWord}
   {dc:DirectCall}
   {asm_op syscall_state : Type}
